\documentclass[20150903-160354-rs2.2-MarksMathNotebook.tex]{subfiles}

\begin{document}
%-=-=-=-=-=-=-=-=-=-=-=-=-=-=-=-=-=-=-=-=-=-=-=-=
%
%	CHAPTER
%
%-=-=-=-=-=-=-=-=-=-=-=-=-=-=-=-=-=-=-=-=-=-=-=-=

\chapter{Simplifying Multivariate Monomials}

%-=-=-=-=-=-=-=-=-=-=-=-=-=-=-=-=-=-=-=-=-=-=-=-=
%	SECTION: Simplifying Degree 0 Multivariate Monomials
%-=-=-=-=-=-=-=-=-=-=-=-=-=-=-=-=-=-=-=-=-=-=-=-=

%-=-=-= DEFINITION
\begin{definition}[Zero Polynomial]\index{Zero Polynomial}\label{zeropolynomial}
A constant polynomial with a value of zero whose coefficients are all equal to zero is called a zero polynomial.  The zero polynomial, 0, can be classified as a degree -1 polynomial.  The zero polynomial is the additive identity, AId \eqref{eq:aid2}, for polynomials.

\hfill \cite{mathworld:zeropolynomial}
\end{definition}


\section{Simplifying Degree -1 Multivariate Monomials}\label{Simplify!Degree -1 Multivariate Monomials}

%-=-=-= EXAMPLE
\begin{example}[id:20151018-165132] \label{20151018-165132}\index{Example!20151018-165132} \hfill \\
Simplify $xy-xy$

\soln

\solnsteps
\begin{align*}
1xy-1xy && \text{MId} \eqref{eq:mid1} \\
1xy + \neg 1 xy && \text{DOS} \eqref{eq:dos1} \\
(1+\neg 1)xy && \text{DPF} \eqref{eq:dpf1} \\
0xy && \text{OOA} \eqref{eq:ooa} \\
0 && \text{AId} \eqref{eq:aid2} 
\end{align*}

\qdepend

\qdependlist
example \ref{20151018-164638}-20151018-164638

\end{example}

\begin{remark}
	This is a special case of a polynomial that is made up of one monomial whose coefficient is equal to zero.  This corresponds to a constant with a value of zero and called the zero polynomial\ref{zeropolynomial}.  The zero polynomial is the additive identity.
\end{remark}

%-=-=-=-=-=-=-=-=-=-=-=-=-=-=-=-=-=-=-=-=-=-=-=-=
%	SECTION:
%-=-=-=-=-=-=-=-=-=-=-=-=-=-=-=-=-=-=-=-=-=-=-=-=
\section{Simplifying Degree 2 Multivariate Monomials}\index{Simplify!Degree 2 Multivariate Monomials}

%-=-=-= EXAMPLE
\begin{example}[id:20151018-161315] \label{20151018-161315}\index{Example!20151018-161315} \hfill \\
Simplify by expanding $4x2y$

\soln

\solnsteps
\begin{align*}
4 \cdot x \cdot 2 \cdot y && \text{JTC} \eqref{eq:jtc} \\
4 \cdot 2 \cdot x \cdot y && \text{CPM} \eqref{eq:cpm} \\
8 \cdot x \cdot y && \text{OOM} \eqref{eq:oom} \\
8xy && \text{CTJ} \eqref{eq:ctj} 
\end{align*}
\end{example}


%-=-=-=-=-=-=-=-=-=-=-=-=-=-=-=-=-=-=-=-=-=-=-=-=
%	SECTION: Simplifying Degree 2 Multivariate Binomials
%-=-=-=-=-=-=-=-=-=-=-=-=-=-=-=-=-=-=-=-=-=-=-=-=

\section{Simplifying Degree 2 Multivariate Binomials}\label{Simplify! Degree 2 Multivariate Binomials}

%-=-=-= EXAMPLE
\begin{example}[id:20151018-164351] \label{20151018-164351}\index{Example!20151018-164351} \hfill \\

Simplify $10xy + 21xy$

\soln

\solnsteps
\begin{align*}
(10+21)xy && \text{DPF} \eqref{eq:dpf1} \\
31xy && \text{OOA} \eqref{eq:ooa} 
\end{align*}

\qdepend

\qdependlist
example \ref{20151018-161544}-20151018-161544

\end{example}


%-=-=-=-=-=-=-=-=-=-=-=-=-=-=-=-=-=-=-=-=-=-=-=-=
%	SECTION: Simplifying Degree 2 Multivariate Trinomials
%-=-=-=-=-=-=-=-=-=-=-=-=-=-=-=-=-=-=-=-=-=-=-=-=

\section{Simplifying Degree 2 Multivariate Trinomials}\label{Simplify! Degree 2 Multivariate Trinomials}

%-=-=-= EXAMPLE
\begin{example}[id:20151018-161544] \label{20151018-161544}\index{Example!20151018-161544} \hfill \\
Simplify by expanding $(2x+3y)(7x+5y)$

\soln

\solnsteps
\begin{align*}
2x(7x+5y) + 3y(7x+5y) && \text{DPE} \eqref{eq:dpe2} \\
2x \cdot 7x + 2x \cdot 5y + 3y \cdot 7x + 3y \cdot 5y && \text{DPE} \eqref{eq:dpe1} \\
2 \cdot x \cdot 7 \cdot x +  2 \cdot x \cdot 5 \cdot y + 3 \cdot y \cdot 7 \cdot x + 3 \cdot y \cdot 5 \cdot y && \text{JTC} \eqref{eq:jtc} \\
2 \cdot 7 \cdot x \cdot x +  2 \cdot 5 \cdot x \cdot y + 3 \cdot 7 \cdot x \cdot y + 3 \cdot 5 \cdot y \cdot y && \text{CPM} \eqref{eq:cpm} \\
2 \cdot 7 \cdot x^2 +  2 \cdot 5 \cdot x \cdot y + 3 \cdot 7 \cdot x \cdot y + 3 \cdot 5 \cdot y^2 && \text{PrCBPo} \eqref{eq:prcbpo1} \\
14 \cdot x^2 +  10 \cdot x \cdot y + 21 \cdot x \cdot y + 15 \cdot y^2 && \text{OOM} \eqref{eq:oom} \\
14x^2 +  10xy + 21xy + 15y^2 && \text{CTJ} \eqref{eq:ctj} \\
14x^2 +  31xy + 15y^2 && \text{OOA} \eqref{eq:ooa} \text{\, goto \,} \, \ref{20151018-164351} 
\end{align*}
\end{example}

%-=-=-= EXAMPLE
\begin{example}[id:20151018-183900] \label{20151018-183900}\index{Example!20151018-183900} \hfill \\
Simplify by expanding $(x+y)^2$

\soln

\solnsteps
\begin{align*}
(1x+1y)^2 && \text{MId} \eqref{eq:mid1} \\
(1x+1y)(1x+1y) && \text{PoTF} \eqref{eq:potf} \\
1x(1x+1y)+ 1y(1x+1y) && \text{DPE} \eqref{eq:dpe2} \\
1x \cdot 1x + 1x \cdot 1y + 1y \cdot 1x + 1y \cdot 1y && \text{DPE} \eqref{eq:dpe1} \\
1 \cdot x \cdot 1 \cdot x + 1 \cdot x \cdot 1 \cdot y + 1 \cdot y \cdot 1 \cdot x + 1 \cdot y \cdot 1 \cdot y && \text{JTC} \eqref{eq:jtc} \\
1 \cdot 1 \cdot x \cdot x + 1 \cdot 1 \cdot x \cdot y + 1 \cdot 1 \cdot x \cdot y + 1 \cdot 1 \cdot y \cdot y && \text{CPM} \eqref{eq:cpm} \\
1 \cdot 1 \cdot x^2 + 1 \cdot 1 \cdot x \cdot y + 1 \cdot 1 \cdot x \cdot y + 1 \cdot 1 \cdot y^2 && \text{PrCBPo} \eqref{eq:prcbpo1} \\
1 \cdot x^2 + 1 \cdot x \cdot y + 1 \cdot x \cdot y + 1 \cdot y^2 && \text{OOM} \eqref{eq:oom} \\
1x^2 + 1xy + 1xy + 1y^2 && \text{CTJ} \eqref{eq:ctj} \\
1x^2 + (1+1)xy + 1y^2 && \text{DPF} \eqref{eq:dpf1} \\
1x^2 + 2xy + 1y^2 && \text{OOA} \eqref{eq:ooa} \\
x^2 + 2xy + y^2 && \text{MId} \eqref{eq:mid2} 
\end{align*}
\end{example}

%-=-=-= EXAMPLE
\begin{example}[id:20151018-182202] \label{20151018-182202}\index{Example!20151018-182202} \hfill \\
Simplify by expanding $(x-y)^2$

\soln

\solnsteps
\begin{align*}
(1x-1y)^2 && \text{MId} \eqref{eq:mid1} \\
(1x-1y)(1x-1y) && \text{PoTF} \eqref{eq:potf} \\
(1x-1y)(1x-1y) && \text{MId} \eqref{eq:mid1} \\
(1x + \neg 1y)(1x + \neg 1y) && \text{DOS} \eqref{eq:dos1} \\
1x(1x+\neg 1y) + \neg 1y(1x+\neg 1y) && \text{DPE} \eqref{eq:dpe2} \\
1x \cdot 1x + 1x \cdot \neg 1y + \neg 1y \cdot 1x + \neg 1y \cdot \neg 1y && \text{DPE} \eqref{eq:dpe1} \\
1 \cdot x \cdot 1 \cdot x + 1 \cdot x \cdot \neg 1 \cdot y + \neg 1 \cdot y \cdot 1 \cdot x + \neg 1 \cdot y \cdot \neg 1 \cdot y && \text{JTC} \eqref{eq:jtc} \\
1 \cdot 1 \cdot x \cdot x + 1 \cdot \neg 1 \cdot x \cdot y + \neg 1 \cdot 1 \cdot x \cdot y + \neg 1 \cdot \neg 1 \cdot y \cdot y && \text{CPM} \eqref{eq:cpm} \\
1 \cdot 1 \cdot x^2 + 1 \cdot \neg 1 \cdot x \cdot y + \neg 1 \cdot 1 \cdot x \cdot y + \neg 1 \cdot \neg 1 \cdot y^2 && \text{PrCBPo} \eqref{eq:prcbpo1} \\
1 \cdot x^2 + \neg 1 \cdot x \cdot y + \neg 1 \cdot x \cdot y + 1 \cdot y^2 && \text{OOM} \eqref{eq:oom} \\
1x^2 + \neg 1xy + \neg 1xy + 1y^2 && \text{CTJ} \eqref{eq:ctj} \\
1x^2 + (\neg 1 + \neg 1)xy + 1y^2 && \text{DPF} \eqref{eq:dpf1} \\
1x^2 + \neg 2xy + 1y^2 && \text{OOA} \eqref{eq:ooa} \\
1x^2 - 2xy + 1y^2 && \text{DOS} \eqref{eq:dos2} \\
x^2-2xy+y^2 && \text{AId} \eqref{eq:aid2} 
\end{align*}
\end{example}

%-=-=-= EXAMPLE
\begin{example}[id:20151018-164638] \label{20151018-164638}\index{Example!20151018-164638} \hfill \\
Simplify by expanding $(x-y)(x+y)$

\soln

\solnsteps
\begin{align*}
(1x-1y)(1x+1y) && \text{MId} \eqref{eq:mid1} \\
(1x+ \neg 1y)(1x+1y) && \text{DOS} \eqref{eq:dos1} \\
1x(1x+1y) + \neg 1y(1x+1y) && \text{DPE} \eqref{eq:dpe2} \\
1x \cdot 1x + 1x \cdot 1y + \neg 1y \cdot 1x + \neg 1y \cdot 1y && \text{DPE} \eqref{eq:dpe1} \\
1 \cdot x \cdot 1 \cdot x + 1 \cdot x \cdot 1 \cdot y + \neg 1 \cdot y \cdot 1 \cdot x + \neg 1 \cdot y \cdot 1 \cdot y && \text{JTC} \eqref{eq:jtc} \\
1 \cdot 1 \cdot x \cdot x + 1 \cdot 1 \cdot x \cdot y + \neg 1 \cdot 1 \cdot x \cdot y + \neg 1 \cdot 1 \cdot y \cdot y && \text{CPM} \eqref{eq:cpm} \\
1 \cdot 1 \cdot x^2 + 1 \cdot 1 \cdot x \cdot y + \neg 1 \cdot 1 \cdot x \cdot y + \neg 1 \cdot 1 \cdot y^2 && \text{PrCBPo} \eqref{eq:prcbpo1} \\
1\cdot x^2 + 1\cdot x \cdot y + \neg 1 \cdot x \cdot y + \neg 1 \cdot y^2 && \text{OOM} \eqref{eq:oom} \\
1x^2 + 1xy + \neg 1xy + \neg 1y^2 && \text{CTJ} \eqref{eq:ctj} \\
1x^2 + \neg 1y^2 && \text{OOA} \eqref{eq:ooa} \text{\, goto \,} \, \ref{20151018-165132}\\
1x^2 - 1y^2 && \text{DOS} \eqref{eq:dos2} \\
x^2-y^2 && \text{MId} \eqref{eq:mid2} 
\end{align*}
\end{example}


\end{document}

